\documentclass{article}%有book，report，letter，article
\title{\heiti the first week}%标题
\author{\kaishu Bingru Yan}% 作者
\date{\today}%时间
\usepackage{ctex}
\newcommand\degree{^\circ}%定义degree命令

\begin{document}
	\maketitle%输出标题、作者和时间
	
	你好，\LaTeX。
	我是中国人，我爱我的祖国。
	I am Chinese; I love my motherland.	
	$$\degree$$
	
	\begin{equation}
		AB^2=BC^2+AC^2
	\end{equation}
	$$(A \cap B) \cup C = $$
	
	$$\{x \mid ~x \in C ~or ~x \in (A \cap B)\} = $$
	
	$$\{x \mid ~x \in C ~or ~(x \in A ~and ~x \in B)\} = $$
	
	$$\{x \mid ~x \in C ~or ~x \in A ~and ~x \in C ~or  ~x \in B\} = $$
	
	$$\{x \mid ~x \in (A \cup C) ~and ~x \in (B \cup C)\} =$$ 
	
	$$(A \cup C) \cap (B \cup C).$$


	Let's define $f(x)$ by the formula $f(x)=x^{e}$.$$f(x)=x^e$$
	
	$ \alpha \in (A\bigcup C)\bigcap (B\bigcup C)$
	
	$\Rightarrow \alpha \in(A\bigcup C) \wedge \alpha \in(B\bigcup C)$
	
	$\Rightarrow (\alpha \in A \wedge \alpha \in B) \vee 
	(\alpha \in A \wedge \alpha \in C) \vee 
	(\alpha \in C \wedge \alpha \in B) \vee 
	(\alpha \in C \wedge \alpha \in C)$
	
	$\Rightarrow \alpha \in (A \bigcap B) \bigcup 
	(A \bigcap C) \bigcup 
	(B \bigcap C) \bigcup 
	(C \bigcap C)$
	
	because $(A \bigcap C) \subset C, (B \bigcap C) \subset C, (C \bigcap C) \subset C$
	
	so $\alpha \in (A \bigcap B) \bigcup 
	(A \bigcap C) \bigcup 
	(B \bigcap C) \bigcup 
	(C \bigcap C)$
	
	
	$\Rightarrow \alpha \in (A \bigcap B) \bigcup C$
	
	so $(A\bigcup C)\bigcap (B\bigcup C) \subset (A \bigcap B) \bigcup C$
	
	step 2:
	
	$(A \bigcap B) \subset A \Rightarrow (A \bigcap B) \bigcup C \subset (A \bigcup C)$

	$(A \bigcap B) \subset B \Rightarrow (A \bigcap B) \bigcup C \subset (B \bigcup C)$
	
	
	
	The 2nd problem
	
	$(\lambda + \mu)x = x^{(\lambda + \mu)}$
	
	$\leq$
\end{document}